src/convert.ml
@@ -1,8 +1,0 @@
-let rec to_nat = function
-  | 0 -> Extract.O
-  | n when n > 0 -> Extract.S (to_nat (n - 1))
-  | _ -> failwith "not a nat"
-
-let rec from_nat = function
-  | Extract.O -> 0
-  | Extract.S n -> 1 + from_nat n
