src/convert.mli
@@ -1,5 +1,0 @@
-(** Convert [int] to [Extract.nat]. **)
-val to_nat : int -> Extract.nat
-
-(** Convert [Extract.nat] to [int]. **)
-val from_nat : Extract.nat -> int
