theories/memory_vec.v
@@ -7,7 +7,7 @@
  *)
 
 From mathcomp Require Import ssreflect ssrbool eqtype seq ssrnat.
-From Coq Require Import BinInt BinNat NArith Lia Uint63.
+From Coq Require Import BinInt BinNat NArith Lia.
 From Wasm Require Import numerics bytes memory common.
 
 Set Implicit Arguments.
@@ -25,110 +25,110 @@ Section Array.
 Context {A: Type}.
   
 Parameter array : Type -> Type.
-Parameter arr_make : PrimInt63.int -> A -> array A.
+Parameter arr_make : N -> A -> array A.
 (* The same as make but initialises its prefix with values from
    the prefix of another array.
    Does not overflow if the length exceeds the make length.
    This is used in the vector_grow function.
  *)
-Parameter arr_make_copy: PrimInt63.int -> A -> array A -> PrimInt63.int -> array A.
-Parameter arr_get : array A -> PrimInt63.int -> A.
+Parameter arr_make_copy: N -> A -> array A -> N -> array A.
+Parameter arr_get : array A -> N -> A.
 Parameter arr_default : array A -> A.
-Parameter arr_set : array A -> PrimInt63.int -> A -> array A.
+Parameter arr_set : array A -> N -> A -> array A.
 (* Takes the length and the generator for the block *)
-Parameter arr_set_gen : array A -> PrimInt63.int -> PrimInt63.int -> (PrimInt63.int -> A) -> array A.
-Parameter arr_length : array A -> PrimInt63.int.
+Parameter arr_set_gen : array A -> N -> N -> (N -> A) -> array A.
+Parameter arr_length : array A -> N.
 Parameter arr_copy : array A -> array A.
 
-Definition max_arr_length : PrimInt63.int := Uint63.of_Z (Z.of_N byte_limit).
+Definition max_arr_length : N := byte_limit.
 
 Notation " t .[ i ] " := (arr_get t i) (at level 5).
 Notation " t .[ i <- a ] " := (arr_set t i a) (at level 5).
 
 Parameter get_out_of_bounds :
-  forall (t : array A) (i : PrimInt63.int),
-    PrimInt63.ltb i (arr_length t) = false -> t.[i] = arr_default t.
+  forall (t : array A) (i : N),
+    N.ltb i (arr_length t) = false -> t.[i] = arr_default t.
 Parameter get_set_same :
-  forall (t : array A) (i : PrimInt63.int) (a : A),
-    PrimInt63.ltb i (arr_length t) = true -> t.[i<-a].[i] = a.
+  forall (t : array A) (i : N) (a : A),
+    N.ltb i (arr_length t) = true -> t.[i<-a].[i] = a.
 Parameter get_set_other :
-  forall (t : array A) (i j : PrimInt63.int) (a : A),
+  forall (t : array A) (i j : N) (a : A),
     i <> j -> t.[i<-a].[j] = t.[j].
 Parameter default_set :
-  forall (t : array A) (i : PrimInt63.int) (a : A),
+  forall (t : array A) (i : N) (a : A),
     arr_default t.[i<-a] = arr_default t.
 Parameter get_make :
-  forall (a : A) (size i : PrimInt63.int),
+  forall (a : A) (size i : N),
     (arr_make size a).[i] = a.
 Parameter get_make_copy:
-  forall (a: A) (size i: PrimInt63.int) (t: array A) (initlen: PrimInt63.int),
-    PrimInt63.ltb i size ->
-    PrimInt63.leb initlen (arr_length t) ->
-    PrimInt63.ltb i (arr_length t) ->
+  forall (a: A) (size i: N) (t: array A) (initlen: N),
+    N.ltb i size ->
+    N.leb initlen (arr_length t) ->
+    N.ltb i (arr_length t) ->
     (arr_make_copy size a t initlen).[i] = t.[i].
 Parameter get_make_copy_default:
-  forall (a: A) (size i: PrimInt63.int) (t: array A) (initlen: PrimInt63.int),
-    PrimInt63.ltb i size ->
-    PrimInt63.leb initlen (arr_length t) ->
-    PrimInt63.leb initlen i ->
+  forall (a: A) (size i: N) (t: array A) (initlen: N),
+    N.ltb i size ->
+    N.leb initlen (arr_length t) ->
+    N.leb initlen i ->
     (arr_make_copy size a t initlen).[i] = a.
 Parameter leb_length :
   forall (t : array A),
-    PrimInt63.leb (arr_length t) max_arr_length = true.
+    N.leb (arr_length t) max_arr_length = true.
 Parameter length_make :
-  forall (size : PrimInt63.int) (a : A),
+  forall (size : N) (a : A),
     arr_length (arr_make size a) =
-      Uint63.min size max_arr_length.
+      N.min size max_arr_length.
 Parameter length_make_copy :
-  forall (size : PrimInt63.int) (a : A) (t: array A) (initlen: PrimInt63.int),
+  forall (size : N) (a : A) (t: array A) (initlen: N),
     arr_length (arr_make_copy size a t initlen) =
-      Uint63.min size max_arr_length.
+      N.min size max_arr_length.
 Parameter length_set :
-  forall (t : array A) (i : PrimInt63.int) (a : A),
+  forall (t : array A) (i : N) (a : A),
     arr_length t.[i<-a] = arr_length t.
 
 (* Some added axioms for set_gen *)
 Parameter length_set_gen :
-  forall (t : array A) (i : PrimInt63.int) (len: PrimInt63.int) (gen: PrimInt63.int -> A),
+  forall (t : array A) (i : N) (len: N) (gen: N -> A),
     arr_length (arr_set_gen t i len gen) = arr_length t.
 
 Parameter arr_set_gen_lookup:
   forall n len gen m i,
-    PrimInt63.ltb i len ->
-    arr_get (arr_set_gen m n len gen) (PrimInt63.add n i) = (gen i).
+    N.ltb i len ->
+    arr_get (arr_set_gen m n len gen) (N.add n i) = (gen i).
 
 Parameter arr_set_gen_lt:
   forall n len gen m i,
-    PrimInt63.ltb i n ->
+    N.ltb i n ->
     arr_get (arr_set_gen m n len gen) i = arr_get m i.
 
 Parameter arr_set_gen_ge:
   forall n len gen m i,
-    PrimInt63.ltb (PrimInt63.add n len) i ->
+    N.ltb (N.add n len) i ->
     arr_get (arr_set_gen m n len gen) i = arr_get m i.
                                          
 Parameter get_copy :
-  forall (t : array A) (i : PrimInt63.int),
+  forall (t : array A) (i : N),
     (arr_copy t).[i] = t.[i].
 Parameter length_copy :
   forall (t : array A), arr_length (arr_copy t) = arr_length t.
 Parameter array_ext :
   forall (t1 t2 : array A),
     arr_length t1 = arr_length t2 ->
-    (forall i : PrimInt63.int,
-        PrimInt63.ltb i (arr_length t1) = true -> t1.[i] = t2.[i]) ->
+    (forall i : N,
+        N.ltb i (arr_length t1) = true -> t1.[i] = t2.[i]) ->
     arr_default t1 = arr_default t2 -> t1 = t2.
 Parameter default_copy :
   forall (t : array A), arr_default (arr_copy t) = arr_default t.
 Parameter default_make :
-  forall (a : A) (size : PrimInt63.int),
+  forall (a : A) (size : N),
     arr_default (arr_make size a) = a.
 Parameter get_set_same_default :
-  forall (t : array A) (i : PrimInt63.int),
+  forall (t : array A) (i : N),
     t.[i<-arr_default t].[i] = arr_default t.
 Parameter get_not_default_lt :
-  forall (t : array A) (x : PrimInt63.int),
-    t.[x] <> arr_default t -> PrimInt63.ltb x (arr_length t) = true.
+  forall (t : array A) (x : N),
+    t.[x] <> arr_default t -> N.ltb x (arr_length t) = true.
 
 End Array.
 
@@ -139,19 +139,13 @@ Section vector.
 
   Implicit Types x : T.
   
-  Definition Uint63_of_N n : PrimInt63.int := Uint63.of_Z (Z.of_N n).
-  Definition Uint63_to_N z : N := Z.to_N (Uint63.to_Z z).
-
-  Definition Uint63_of_positive p : PrimInt63.int := Uint63.of_Z (Zpos p).
-  Definition Uint63_to_positive z : positive := Z.to_pos (Uint63.to_Z z).
-  
   Record vector :=
     { v_data: array T;
       v_size: N;
       v_capacity: N;
       v_init: T;
       v_size_valid: v_size <= v_capacity;
-      v_capacity_eq: v_capacity = Uint63_to_N (arr_length v_data);
+      v_capacity_eq: v_capacity = (arr_length v_data);
     }.
 
   Definition vector_length vec : N :=
@@ -160,27 +154,23 @@ Section vector.
   Definition vector_make (len: N) x : vector.
   Proof.
     remember (N.min len byte_limit) as capped_len.
-    refine (@Build_vector (arr_make (Uint63_of_N capped_len) x) capped_len capped_len x _ _).
+    refine (@Build_vector (arr_make capped_len x) capped_len capped_len x _ _).
     - by lias.
     - rewrite length_make; subst.
-      unfold max_arr_length, Uint63_to_N, Uint63_of_N.
-      rewrite Uint63.min_spec Znat.Z2N.inj_min.
-      repeat rewrite of_Z_spec.
-      repeat rewrite Znat.Z2N.inj_mod => //; try by lias.
-      repeat rewrite Znat.N2Z.id.
-      rewrite N.mod_small; cbn; by lias.
+      unfold max_arr_length.
+      by lias.
   Defined.
     
   Definition vector_lookup vec n : option T :=
     if N.ltb n (vector_length vec) then
-      Some (arr_get vec.(v_data) (Uint63_of_N n))
+      Some (arr_get vec.(v_data) n)
     else None.
 
   Definition vector_update (vec: vector) (n: N) (x: T) : option vector.
   Proof.
     refine
     (if N.ltb n (vector_length vec) then
-      Some (@Build_vector (arr_set vec.(v_data) (Uint63_of_N n) x) vec.(v_size) vec.(v_capacity) vec.(v_init) _ _)
+      Some (@Build_vector (arr_set vec.(v_data) n x) vec.(v_size) vec.(v_capacity) vec.(v_init) _ _)
      else None).
     - by apply v_size_valid.
     - rewrite length_set.
@@ -191,7 +181,7 @@ Section vector.
   Proof.
     refine
     (if N.leb (N.add n len) (vector_length vec) then
-      Some (@Build_vector (arr_set_gen vec.(v_data) (Uint63_of_N n) (Uint63_of_N len) (fun offset => gen (Uint63_to_N offset))) vec.(v_size) vec.(v_capacity) vec.(v_init) _ _)
+      Some (@Build_vector (arr_set_gen vec.(v_data) n len (fun offset => gen offset)) vec.(v_size) vec.(v_capacity) vec.(v_init) _ _)
      else None).
     - by apply v_size_valid.
     - rewrite length_set_gen.
@@ -214,7 +204,7 @@ Section vector.
         | false =>
             let new_capacity := (N.min (N.max newsize (vec.(v_capacity) * 2%N)) byte_limit) in
             let x := vec.(v_init) in
-            let new_vd := arr_make_copy (Uint63_of_N new_capacity) x vec.(v_data) (Uint63_of_N vec.(v_size)) in
+            let new_vd := arr_make_copy new_capacity x vec.(v_data) vec.(v_size) in
             (fun _ => Some (@Build_vector new_vd newsize new_capacity x _ _))
         end (Logic.eq_refl (newsize <=? vec.(v_capacity))))
     | false => (fun _ => None)
@@ -231,11 +221,8 @@ Section vector.
   Qed.
   Next Obligation.
     rewrite length_make_copy.
-    unfold Uint63_to_N, Uint63_of_N.
-    rewrite min_spec Znat.Z2N.inj_min of_Z_spec.
-    rewrite Znat.Z2N.inj_mod; try by lias.
-    rewrite Znat.N2Z.id.
-    rewrite N.mod_small; cbn; by lias.
+    unfold max_arr_length.
+    by lias.
   Qed.
 
   Lemma vector_size_bound: forall vec,
@@ -244,9 +231,8 @@ Section vector.
     move => vec.
     specialize (@v_size_valid vec) as Hvalid.
     specialize (v_capacity_eq vec) as Hcap.
-    unfold Uint63_to_N in Hcap.
     rewrite Hcap in Hvalid.
-    specialize (leb_length (v_data vec)) as Hlenub; move/Uint63.lebP in Hlenub.
+    specialize (leb_length (v_data vec)) as Hlenub; move/N.leb_spec0 in Hlenub.
     unfold max_arr_length in Hlenub.
     clear Hcap.
     cbn in *; by lias.
@@ -334,20 +320,7 @@ Qed.
     unfold vector_length in Hif.
     specialize (v_capacity_eq mem) as Hcap.
     specialize (@v_size_valid _ mem) as Hsize.
-    move/N.ltb_spec0 in Hif.
-    apply/ltbP.
-    unfold Uint63_of_N.
-    unfold Uint63_to_N in Hcap.
-    rewrite of_Z_spec.
-    apply (f_equal Z.of_N) in Hcap.
-    rewrite Znat.Z2N.id in Hcap.
-    - rewrite - Hcap.
-      assert (Z.of_N i mod wB <= Z.of_N i)%Z as Hbound.
-      { apply Z.mod_le; by lias. }
-      (* lots of transitivity *)
-      by lias.
-    - specialize (to_Z_bounded (arr_length (v_data mem))).
-      by lias.
+    by lias.
   Qed.
 
 Lemma mv_update_lookup_ne:
@@ -364,17 +337,6 @@ Proof.
   unfold vector_length.
   destruct (i <? v_size mem) eqn:Hindex => //.
   rewrite get_set_other => //.
-  unfold Uint63_of_N.
-  move => Hinjeq.
-  unfold vector_length in Hif.
-  move/N.ltb_spec0 in Hindex.
-  specialize (@vector_size_bound _ mem) as Hsizebound.
-  assert (i < byte_limit) as Hiub; first by lias.
-  assert (j < byte_limit) as Hjub; first by lias.
-  apply (f_equal to_Z) in Hinjeq.
-  do 2 (rewrite of_Z_spec in Hinjeq).
-  cbn in *.
-  do 2 (rewrite Z.mod_small in Hinjeq => //; last by lias).
   by lias.
 Qed.
   
@@ -497,24 +459,9 @@ Proof.
     assert (i < byte_limit) as Hibound; first by lias.
     specialize (@v_size_valid _ mem) as Hsize.
     specialize (v_capacity_eq mem) as Hcap.
-    unfold Uint63_to_N in Hcap.
     rewrite Hcap in Hsize.
-    apply Znat.N2Z.inj_le in Hsize.
-    specialize (to_Z_bounded (arr_length (v_data mem))) as HZbound.
-    rewrite Znat.Z2N.id in Hsize => //; last by lias.
-    rewrite get_make_copy => //; unfold Uint63_of_N.
-    + apply/Uint63.ltbP.
-      repeat rewrite of_Z_spec.
-      do 2 (rewrite Z.mod_small; last by cbn; cbn in Hub; lias).
-      by lias.
-    + apply/Uint63.lebP.
-      rewrite of_Z_spec.
-      rewrite Z.mod_small; by lias.
-    + apply/Uint63.ltbP.
-      rewrite of_Z_spec.
-      rewrite Z.mod_small; last by cbn; cbn in Hibound; lias.
-      unfold vector_length in Hlen.
-      by lias.
+    unfold vector_length in Hlen.
+    rewrite get_make_copy => //; by lias.
 Qed.
   
 #[export]
