src/extraction.v
@@ -1,14 +1,6 @@
 (** Extraction to OCaml. **)
 
 From Coq Require Extraction.
-From Coq Require PArray.
-From Coq Require Import
-  extraction.ExtrOcamlBasic
-  extraction.ExtrOcamlNativeString
-  extraction.ExtrOcamlZBigInt
-  ExtrOCamlInt63
-.
-
 From Wasm Require Import
   efficient_extraction
   datatypes_properties
@@ -24,8 +16,29 @@ From Wasm Require Import
 .
 
 Require Import compcert.lib.Integers.
+Require Import ZArith NArith.
+
+From Coq Require PArray.
+From Coq Require Import
+  extraction.ExtrOcamlBasic
+  extraction.ExtrOcamlNativeString
+  extraction.ExtrOcamlNatInt
+  extraction.ExtrOcamlZInt
+.
 
 Extraction Language OCaml.
+
+Extract Inductive positive => "Coq_types.ocaml_int"
+[ "(fun p->1+2*p)" "(fun p->2*p)" "1" ]
+"(fun f2p1 f2p f1 p -> if p<=1 then f1 () else if p mod 2 = 0 then f2p (p/2) else f2p1 (p/2))".
+
+Extract Inductive Z => "Coq_types.ocaml_int"
+[ "0" "" "(~-)" ]
+"(fun f0 fp fn z -> if z=0 then f0 () else if z>0 then fp z else fn (-z))".
+
+Extract Inductive N => "Coq_types.ocaml_int"
+[ "0" "" ]
+"(fun f0 fp n -> if n=0 then f0 () else fp n)".
 
 Extract Constant lookup_N => "EfficientExtraction.lookup_N_safe".
 
